libcrux-ml-kem/proofs/fstar/extraction/Libcrux_ml_kem.Ind_cca.Multiplexing.fst
@@ -3,29 +3,6 @@ module Libcrux_ml_kem.Ind_cca.Multiplexing
 open Core
 open FStar.Mul
 
-let validate_public_key
-      (v_K v_RANKED_BYTES_PER_RING_ELEMENT v_PUBLIC_KEY_SIZE: usize)
-      (public_key: t_Array u8 v_PUBLIC_KEY_SIZE)
-     =
-  if Libcrux_platform.Platform.simd256_support ()
-  then
-    Libcrux_ml_kem.Ind_cca.Instantiations.Avx2.validate_public_key v_K
-      v_RANKED_BYTES_PER_RING_ELEMENT
-      v_PUBLIC_KEY_SIZE
-      public_key
-  else
-    if Libcrux_platform.Platform.simd128_support ()
-    then
-      Libcrux_ml_kem.Ind_cca.Instantiations.Neon.validate_public_key v_K
-        v_RANKED_BYTES_PER_RING_ELEMENT
-        v_PUBLIC_KEY_SIZE
-        public_key
-    else
-      Libcrux_ml_kem.Ind_cca.Instantiations.Portable.validate_public_key v_K
-        v_RANKED_BYTES_PER_RING_ELEMENT
-        v_PUBLIC_KEY_SIZE
-        public_key
-
 let decapsulate
       (v_K v_SECRET_KEY_SIZE v_CPA_SECRET_KEY_SIZE v_PUBLIC_KEY_SIZE v_CIPHERTEXT_SIZE v_T_AS_NTT_ENCODED_SIZE v_C1_SIZE v_C2_SIZE v_VECTOR_U_COMPRESSION_FACTOR v_VECTOR_V_COMPRESSION_FACTOR v_C1_BLOCK_SIZE v_ETA1 v_ETA1_RANDOMNESS_SIZE v_ETA2 v_ETA2_RANDOMNESS_SIZE v_IMPLICIT_REJECTION_HASH_INPUT_SIZE:
           usize)
@@ -114,3 +91,26 @@ let generate_keypair
         v_ETA1
         v_ETA1_RANDOMNESS_SIZE
         randomness
+
+let validate_public_key
+      (v_K v_RANKED_BYTES_PER_RING_ELEMENT v_PUBLIC_KEY_SIZE: usize)
+      (public_key: t_Array u8 v_PUBLIC_KEY_SIZE)
+     =
+  if Libcrux_platform.Platform.simd256_support ()
+  then
+    Libcrux_ml_kem.Ind_cca.Instantiations.Avx2.validate_public_key v_K
+      v_RANKED_BYTES_PER_RING_ELEMENT
+      v_PUBLIC_KEY_SIZE
+      public_key
+  else
+    if Libcrux_platform.Platform.simd128_support ()
+    then
+      Libcrux_ml_kem.Ind_cca.Instantiations.Neon.validate_public_key v_K
+        v_RANKED_BYTES_PER_RING_ELEMENT
+        v_PUBLIC_KEY_SIZE
+        public_key
+    else
+      Libcrux_ml_kem.Ind_cca.Instantiations.Portable.validate_public_key v_K
+        v_RANKED_BYTES_PER_RING_ELEMENT
+        v_PUBLIC_KEY_SIZE
+        public_key
