libcrux-ml-kem/proofs/fstar/extraction/Libcrux_ml_kem.Ind_cca.Multiplexing.fsti
@@ -3,16 +3,6 @@ module Libcrux_ml_kem.Ind_cca.Multiplexing
 open Core
 open FStar.Mul
 
-val validate_public_key
-      (v_K v_RANKED_BYTES_PER_RING_ELEMENT v_PUBLIC_KEY_SIZE: usize)
-      (public_key: t_Array u8 v_PUBLIC_KEY_SIZE)
-    : Prims.Pure bool
-      (requires
-        Spec.MLKEM.is_rank v_K /\
-        v_RANKED_BYTES_PER_RING_ELEMENT == Spec.MLKEM.v_RANKED_BYTES_PER_RING_ELEMENT v_K /\
-        v_PUBLIC_KEY_SIZE == Spec.MLKEM.v_CCA_PUBLIC_KEY_SIZE v_K)
-      (fun _ -> Prims.l_True)
-
 val decapsulate
       (v_K v_SECRET_KEY_SIZE v_CPA_SECRET_KEY_SIZE v_PUBLIC_KEY_SIZE v_CIPHERTEXT_SIZE v_T_AS_NTT_ENCODED_SIZE v_C1_SIZE v_C2_SIZE v_VECTOR_U_COMPRESSION_FACTOR v_VECTOR_V_COMPRESSION_FACTOR v_C1_BLOCK_SIZE v_ETA1 v_ETA1_RANDOMNESS_SIZE v_ETA2 v_ETA2_RANDOMNESS_SIZE v_IMPLICIT_REJECTION_HASH_INPUT_SIZE:
           usize)
@@ -66,4 +56,14 @@ val generate_keypair
         v_RANKED_BYTES_PER_RING_ELEMENT == Spec.MLKEM.v_RANKED_BYTES_PER_RING_ELEMENT v_K /\
         v_ETA1 == Spec.MLKEM.v_ETA1 v_K /\
         v_ETA1_RANDOMNESS_SIZE == Spec.MLKEM.v_ETA1_RANDOMNESS_SIZE v_K)
+      (fun _ -> Prims.l_True)
+
+val validate_public_key
+      (v_K v_RANKED_BYTES_PER_RING_ELEMENT v_PUBLIC_KEY_SIZE: usize)
+      (public_key: t_Array u8 v_PUBLIC_KEY_SIZE)
+    : Prims.Pure bool
+      (requires
+        Spec.MLKEM.is_rank v_K /\
+        v_RANKED_BYTES_PER_RING_ELEMENT == Spec.MLKEM.v_RANKED_BYTES_PER_RING_ELEMENT v_K /\
+        v_PUBLIC_KEY_SIZE == Spec.MLKEM.v_CCA_PUBLIC_KEY_SIZE v_K)
       (fun _ -> Prims.l_True)
