libcrux-ml-kem/proofs/fstar/extraction/Libcrux_ml_kem.Mlkem1024.fst
@@ -3,21 +3,6 @@ module Libcrux_ml_kem.Mlkem1024
 open Core
 open FStar.Mul
 
-let validate_public_key (public_key: Libcrux_ml_kem.Types.t_MlKemPublicKey (sz 1568)) =
-  if
-    Libcrux_ml_kem.Ind_cca.Multiplexing.validate_public_key (sz 4)
-      (sz 1536)
-      (sz 1568)
-      public_key.Libcrux_ml_kem.Types.f_value
-  then
-    Core.Option.Option_Some public_key
-    <:
-    Core.Option.t_Option (Libcrux_ml_kem.Types.t_MlKemPublicKey (sz 1568))
-  else
-    Core.Option.Option_None
-    <:
-    Core.Option.t_Option (Libcrux_ml_kem.Types.t_MlKemPublicKey (sz 1568))
-
 let decapsulate
       (private_key: Libcrux_ml_kem.Types.t_MlKemPrivateKey (sz 3168))
       (ciphertext: Libcrux_ml_kem.Types.t_MlKemCiphertext (sz 1568))
@@ -54,3 +39,18 @@ let generate_key_pair (randomness: t_Array u8 (sz 64)) =
   in
   let _:Prims.unit = admit () (* Panic freedom *) in
   result
+
+let validate_public_key (public_key: Libcrux_ml_kem.Types.t_MlKemPublicKey (sz 1568)) =
+  if
+    Libcrux_ml_kem.Ind_cca.Multiplexing.validate_public_key (sz 4)
+      (sz 1536)
+      (sz 1568)
+      public_key.Libcrux_ml_kem.Types.f_value
+  then
+    Core.Option.Option_Some public_key
+    <:
+    Core.Option.t_Option (Libcrux_ml_kem.Types.t_MlKemPublicKey (sz 1568))
+  else
+    Core.Option.Option_None
+    <:
+    Core.Option.t_Option (Libcrux_ml_kem.Types.t_MlKemPublicKey (sz 1568))
