libcrux-ml-kem/proofs/fstar/extraction/Libcrux_ml_kem.Mlkem1024.fsti
@@ -62,13 +62,6 @@ let v_CPA_PKE_CIPHERTEXT_SIZE_1024_: usize = v_C1_SIZE_1024_ +! v_C2_SIZE_1024_
 let v_IMPLICIT_REJECTION_HASH_INPUT_SIZE: usize =
   Libcrux_ml_kem.Constants.v_SHARED_SECRET_SIZE +! v_CPA_PKE_CIPHERTEXT_SIZE_1024_
 
-/// Validate a public key.
-/// Returns `Some(public_key)` if valid, and `None` otherwise.
-val validate_public_key (public_key: Libcrux_ml_kem.Types.t_MlKemPublicKey (sz 1568))
-    : Prims.Pure (Core.Option.t_Option (Libcrux_ml_kem.Types.t_MlKemPublicKey (sz 1568)))
-      Prims.l_True
-      (fun _ -> Prims.l_True)
-
 /// Decapsulate ML-KEM 1024
 /// Generates an [`MlKemSharedSecret`].
 /// The input is a reference to an [`MlKem1024PrivateKey`] and an [`MlKem1024Ciphertext`].
@@ -117,3 +110,10 @@ val generate_key_pair (randomness: t_Array u8 (sz 64))
             Spec.MLKEM.Instances.mlkem1024_generate_keypair randomness
           in
           valid ==> (res.f_sk.f_value == secret_key /\ res.f_pk.f_value == public_key))
+
+/// Validate a public key.
+/// Returns `Some(public_key)` if valid, and `None` otherwise.
+val validate_public_key (public_key: Libcrux_ml_kem.Types.t_MlKemPublicKey (sz 1568))
+    : Prims.Pure (Core.Option.t_Option (Libcrux_ml_kem.Types.t_MlKemPublicKey (sz 1568)))
+      Prims.l_True
+      (fun _ -> Prims.l_True)
