libcrux-ml-kem/proofs/fstar/extraction/Libcrux_ml_kem.Vector.Avx2.Serialize.fsti
@@ -19,7 +19,9 @@ val deserialize_12_ (bytes: t_Slice u8)
     : Prims.Pure Libcrux_intrinsics.Avx2_extract.t_Vec256 Prims.l_True (fun _ -> Prims.l_True)
 
 val deserialize_4_ (bytes: t_Slice u8)
-    : Prims.Pure Libcrux_intrinsics.Avx2_extract.t_Vec256 Prims.l_True (fun _ -> Prims.l_True)
+    : Prims.Pure Libcrux_intrinsics.Avx2_extract.t_Vec256
+      (requires (Core.Slice.impl__len #u8 bytes <: usize) =. sz 8)
+      (fun _ -> Prims.l_True)
 
 val deserialize_5_ (bytes: t_Slice u8)
     : Prims.Pure Libcrux_intrinsics.Avx2_extract.t_Vec256 Prims.l_True (fun _ -> Prims.l_True)
@@ -37,7 +39,9 @@ val serialize_5_ (vector: Libcrux_intrinsics.Avx2_extract.t_Vec256)
     : Prims.Pure (t_Array u8 (sz 10)) Prims.l_True (fun _ -> Prims.l_True)
 
 val serialize_4_ (vector: Libcrux_intrinsics.Avx2_extract.t_Vec256)
-    : Prims.Pure (t_Array u8 (sz 8)) Prims.l_True (fun _ -> Prims.l_True)
+    : Prims.Pure (t_Array u8 (sz 8))
+      (requires BitVec.Intrinsics.forall_bool #256 (fun i -> i % 16 < 4 || vector i = 0))
+      (fun _ -> Prims.l_True)
 
 val deserialize_11_ (bytes: t_Slice u8)
     : Prims.Pure Libcrux_intrinsics.Avx2_extract.t_Vec256 Prims.l_True (fun _ -> Prims.l_True)
